defined refinement of CompM specifications, including existential and universal specs, and added rules for proving refinements, including one rule for the either combinator that depends on SAWCorePrelude and so is in its own file CompMExtra.v

coq/handwritten/CryptolToCoq/CompM.v
@@ -58,6 +58,7 @@ Class MonadFixOp (M:Type -> Type) : Type :=
                        (forall (a:A), M (B a)).
 
 (* Typeclass for dependent functions that respect the domain order *)
+(* FIXME: this doesn't need to be a typeclass *)
 Class ProperFixFun {A B M} `{MonadLeqOp M}
       (F:(forall (a:A), M (B a)) -> (forall (a:A), M (B a))) : Prop :=
   { properFixFun : forall f1 f2, (forall a, leqM (f1 a) (f2 a)) ->
@@ -260,6 +261,144 @@ Qed.
 
 
 (***
+ *** The Set of Sets Monad
+ ***)
+
+(*
+FIXME: can we get this to work as a predicate monad for SetM?
+- The hard part is defining bindM: the current version fails associativity
+  because it requires finding a choice function
+- I could imagine P >> Q is the union over all Q a for any a in mA in P, or the
+  union_(s in P) (intersection_(a in s) (Q a))
+- But all of these have issues!
+- e.g., if P contains the empty set, so should P >>= Q!
+
+(* A SetSetM computation is a set of subsets of a type *)
+Definition SetSetM (A:Type) := SetM A -> Prop.
+
+(* Close off a SetSetM under extensional equivalence *)
+Definition inSetSetM {A} (P:SetSetM A) : SetSetM A :=
+  fun m => exists2 m', m' ~= m & P m'.
+
+(* Equivalence of two sets = they contain the same elements *)
+Instance MonadEqOp_SetSetM : MonadEqOp SetSetM :=
+  fun A P1 P2 => forall m, inSetSetM P1 m <-> inSetSetM P2 m.
+
+Instance Proper_eqM_inSetSetM {A} :
+  Proper (eqM ==> eqM ==> iff) (inSetSetM (A:=A)).
+Proof.
+  intros P1 P2 eqP m1 m2 eqm.
+  split; intros [ m' eq_m' in_m' ]; apply eqP; exists m'; try assumption.
+  - transitivity m1; assumption.
+  - transitivity m2; [ | symmetry ]; assumption.
+Qed.
+
+Instance Equivalence_SetSetM_eqM A : Equivalence (eqM (M:=SetSetM) (A:=A)).
+Proof.
+  split.
+  { intros m a; reflexivity. }
+  { intros m1 m2 eq_m a. symmetry. apply eq_m. }
+  { intros m1 m2 m3 eq12 eq23 a. etransitivity; [ apply eq12 | apply eq23 ]. }
+Qed.
+
+Instance MonadReturnOp_SetSetM : MonadReturnOp SetSetM :=
+  fun A a m => m ~= returnM a.
+
+Lemma SetSetM_returnM A (m:SetM A) a :
+  inSetSetM (returnM a) m <-> m ~= returnM a.
+Proof.
+  split.
+  - intros [ m' eq_m' in_P ]. transitivity m'; [ symmetry; assumption | apply in_P ].
+  - intro e_m; exists (returnM a); [ symmetry; assumption | intro; reflexivity ].
+Qed.
+
+Instance MonadBindOp_SetSetM : MonadBindOp SetSetM :=
+  fun A B P Q m =>
+    exists2 mA, inSetSetM P mA &
+                exists2 f, (forall a, mA a -> inSetSetM (Q a) (f a)) &
+                           m ~= mA >>= f.
+
+Lemma SetSetM_bindM_elim {A B P} {Q:A -> SetSetM B} {m} :
+  inSetSetM (P >>= Q) m ->
+  exists2 mA, inSetSetM P mA &
+              exists2 f, (forall a, mA a -> inSetSetM (Q a) (f a)) & m ~= mA >>= f.
+Proof.
+  intros [ m' eq_m [ mA in_P_mA [ f in_Q_f eq_m' ]]].
+  exists mA; [ assumption | ].
+  exists f; [ apply in_Q_f | ].
+  rewrite <- eq_m; assumption.
+Qed.
+
+
+Lemma SetSetM_bindM_intro {A B P} {Q:A -> SetSetM B} {m} mA f :
+  inSetSetM P mA -> (forall a, mA a -> inSetSetM (Q a) (f a)) -> m ~= mA >>= f ->
+  inSetSetM (P >>= Q) m.
+Proof.
+  intros [ mA' eq_mA in_mA' ] in_Q_f eq_m.
+  exists (mA >>= f); [ symmetry; assumption | ].
+  exists mA; [ exists mA'; assumption | ].
+  exists f; [ | reflexivity ]. apply in_Q_f.
+Qed.
+
+Instance Monad_SetSetM : Monad SetSetM.
+Proof.
+  split; intros.
+  { typeclasses eauto. }
+  { intros P1 P2 RP Q1 Q2 RQ m; split;
+      intros [ m' eq_m [ mA in_P_mA [ f in_Q_f eq_m' ] ] ];
+      exists m'; try assumption; exists mA; try (apply RP; assumption);
+        exists f; try assumption;
+          intros a in_mA; apply (RQ a a eq_refl); apply in_Q_f; assumption. }
+  { intro m; split.
+    { intro in_m.
+      destruct (SetSetM_bindM_elim in_m) as [ mA in_mA [ g in_g eq_m ]].
+      rewrite eq_m.
+      rewrite SetSetM_returnM in in_mA. rewrite in_mA. rewrite returnM_bindM.
+      apply in_g. rewrite (in_mA a). apply eq_refl. }
+    { intro in_m. apply (SetSetM_bindM_intro (returnM a) (fun _ => m)).
+      - apply SetSetM_returnM; reflexivity.
+      - intros a' eq_a_a'; compute in eq_a_a'. rewrite <- eq_a_a'. assumption.
+      - rewrite returnM_bindM. reflexivity. } }
+  { intro s; split.
+    { intro in_s.
+      destruct (SetSetM_bindM_elim in_s) as [ mA in_mA [ g in_g eq_s ]].
+      assert (eq_s_mA : s ~= mA); [ | rewrite eq_s_mA; assumption ].
+      transitivity (mA >>= g); [ assumption | ].
+      transitivity (mA >>= returnM); [ | apply bindM_returnM ].
+      intro a; split; intros [ a' in_a' in_f_a' ]; exists a'; try assumption.
+      - destruct (in_g a' in_a') as [ s' eq_s' in_s'].
+        rewrite <- (in_s' a). rewrite (eq_s' a). assumption.
+      - destruct (in_g a' in_a')  as [ s' eq_s' in_s'].
+        rewrite <- (eq_s' a). apply in_s'. assumption. }
+    { intros [ s' eq_s' in_m_s' ]. exists s'; [ assumption | ].
+      exists s'; [ exists s'; [ reflexivity | assumption ] | ].
+      exists returnM; [ | symmetry; apply bindM_returnM ].
+      intros a in_s'. exists (returnM a); [ reflexivity | ].
+      intro a'; reflexivity. } }
+  { intro sC; split; intro in_sC.
+    { destruct (SetSetM_bindM_elim in_sC) as [ sB in_sB [ sg in_sg eq_sC ]].
+      destruct (SetSetM_bindM_elim in_sB) as [ sA in_sA [ sf in_sf eq_sB ]].
+      apply (SetSetM_bindM_intro sA (fun x => sf x >>= sg)); try assumption;
+        [ | rewrite eq_sC; rewrite eq_sB; rewrite bindM_bindM; reflexivity ].
+      intros a in_a.
+      apply (SetSetM_bindM_intro (sf a) sg); [ apply in_sf; assumption | | reflexivity ].
+      intros b in_b. apply in_sg. rewrite (eq_sB b).
+      exists a; assumption. }
+    { destruct (SetSetM_bindM_elim in_sC) as [ sA in_sA [ sfg in_sfg eq_sC ]].
+      apply (SetSetM_bindM_intro sA sfg).
+
+
+      admit. } }
+
+      apply (SetSetM_bindM_intro sA sfg); try assumption.
+
+      destruct (SetSetM_bindM_elim in_sB) as [ sA in_sA [ sf in_sf eq_sB ]].
+
+    intros [ sC' eq_sC' [ sB [ sB' eq_sB' [ sA eq_sA in_sA ] ] eq_sB ] ]. destruct in_sC'.
+ *)
+
+
+(***
  *** The Computation Monad = the Option-Set Monad
  ***)
 
@@ -384,3 +523,152 @@ Definition multiFixM {lrts:LetRecTypes}
 Definition letRecM {lrts : LetRecTypes} {B} (F: lrtPi lrts (lrtTupleType lrts))
            (body:lrtPi lrts (CompM B)) : CompM B :=
   lrtApply body (multiFixM F).
+
+
+(* FIXME: write this! *)
+Class ProperLRTFun {lrts} (F : lrtPi lrts (lrtTupleType lrts)) : Prop :=
+  { properLRTFun : True }.
+
+Instance ProperLRTFun_any lrts F : @ProperLRTFun lrts F.
+Proof.
+  constructor. apply I.
+Qed.
+
+
+(***
+ *** Refinement Proofs
+ ***)
+
+Definition refinesM {A} (m1 m2:CompM A) : Prop := forall a, m1 a -> m2 a.
+
+Infix "|=" := refinesM (at level 70, no associativity).
+
+Instance PreOrder_refinesM A : PreOrder (refinesM (A:=A)).
+Proof.
+  split.
+  { intros m a in_a; assumption. }
+  { intros m1 m2 m3 R12 R23 a in_m1. apply R23. apply R12. assumption. }
+Qed.
+
+Instance Proper_eqM_refinesM A : Proper (eqM ==> eqM ==> iff) (refinesM (A:=A)).
+Proof.
+  intros m1 m1' e1 m2 m2' e2.
+  split; intros R12 a in_a; apply e2; apply R12; apply e1; assumption.
+Qed.
+
+Instance Proper_refinesM_bindM A B :
+  Proper (refinesM ==> (eq ==> refinesM) ==> refinesM) (bindM (A:=A) (B:=B)).
+Proof.
+  intros m1 m2 Rm f1 f2 Rf opt_b [ opt_a in_opt_a in_opt_b ].
+  exists opt_a; [ apply Rm; assumption | ].
+  destruct opt_a; [ | assumption ].
+  apply (Rf a a eq_refl); assumption.
+Qed.
+
+
+(* If a monadic function f is F-closed w.r.t. the refinement relation, then the
+least fixed-point of F refines f *)
+Lemma refinesM_fixM A B (F : (forall (a:A), CompM (B a)) ->
+                             (forall (a:A), CompM (B a))) f :
+  (forall a, F f a |= f a) -> forall a, fixM F a |= f a.
+Proof.
+  admit. (* FIXME *)
+Admitted.
+
+(* Lift refinesM to monadic functions *)
+Fixpoint refinesFun {lrt} : relation (lrtToType lrt) :=
+  match lrt return relation (lrtToType lrt) with
+  | LRT_Ret B => refinesM
+  | LRT_Fun A lrtF => fun f1 f2 => forall a, refinesFun (f1 a) (f2 a)
+  end.
+
+(* Lift refinesM to tuples of monadic functions *)
+Fixpoint refinesFunTuple {lrts} : relation (lrtTupleType lrts) :=
+  match lrts return relation (lrtTupleType lrts) with
+  | LRT_Nil => fun _ _ => True
+  | LRT_Cons lrt lrts' =>
+    fun tup1 tup2 => refinesFun (fst tup1) (fst tup2) /\
+                     refinesFunTuple (snd tup1) (snd tup2)
+  end.
+
+Lemma refinesFunTuple_multiFixM lrts (F:lrtPi lrts (lrtTupleType lrts)) tup :
+  refinesFunTuple (lrtApply F tup) tup -> refinesFunTuple (multiFixM F) tup.
+Proof.
+  admit. (* FIXME *)
+Admitted.
+
+Lemma refinesFun_multiFixM_fst lrt (F:lrtPi (LRT_Cons lrt LRT_Nil)
+                                            (lrtTupleType (LRT_Cons lrt LRT_Nil))) f
+      (ref_f:refinesFun (fst (F f)) f) :
+  refinesFun (fst (multiFixM F)) f.
+Proof.
+  refine (proj1 (refinesFunTuple_multiFixM (LRT_Cons lrt LRT_Nil) _ (f, tt) _)).
+  split; [ | constructor ].
+  apply ref_f.
+Qed.
+
+
+Lemma refinesM_if {A} (m1 m2:CompM A) b P :
+  (b = true -> m1 |= P) -> (b = false -> m2 |= P) ->
+  (if b then m1 else m2) |= P.
+Proof.
+  intros ref1 ref2; destruct b; [ apply ref1 | apply ref2 ]; reflexivity.
+Qed.
+
+Lemma simpl_letRecM0 B F body : @letRecM LRT_Nil B F body = body.
+Proof.
+  reflexivity.
+Qed.
+
+Lemma refinesM_sigT_rect {A1 A2 B} F P (s: {x:A1 & A2 x}) :
+  (forall a1 a2, s = existT _ a1 a2 -> F a1 a2 |= P) ->
+  sigT_rect (fun _ => CompM B) F s |= P.
+Proof.
+  destruct s; intros.
+  apply H. reflexivity.
+Qed.
+
+
+(** Existential Specifications **)
+
+Definition existsM {A B} (P: A -> CompM B) : CompM B :=
+  fun b => exists a, P a b.
+
+Lemma refinesM_existsM_r {A B} (P: A -> CompM B) m a :
+  m |= (P a) -> m |= (existsM P).
+Proof.
+  intros r b in_b. exists a. apply r. assumption.
+Qed.
+
+Lemma refinesM_existsM_l A B (P: A -> CompM B) Q :
+  (forall a, P a |= Q) -> existsM P |= Q.
+Proof.
+  intros r b [ a in_b ]. apply (r a). assumption.
+Qed.
+
+Lemma existsM_bindM A B C (P: A -> CompM B) (Q: B -> CompM C) :
+  (existsM P) >>= Q ~= existsM (fun x => P x >>= Q).
+Proof.
+  intros c; split.
+  - intros [ opt_b [ a in_b ] in_c ]. exists a. exists opt_b; assumption.
+  - intros [ a [ opt_b in_b in_c ] ]. exists opt_b; [ | assumption ].
+    exists a; assumption.
+Qed.
+
+
+(** Universal Specifications **)
+
+Definition forallM {A B} (P: A -> CompM B) : CompM B :=
+  fun b => forall a, P a b.
+
+Lemma refinesM_forallM_r {A B} P (Q: A -> CompM B) :
+  (forall a, P |= (Q a)) -> P |= (forallM Q).
+Proof.
+  intros r b in_b a. apply r. assumption.
+Qed.
+
+Lemma refinesM_forallM_l {A B} (P: A -> CompM B) Q a :
+  P a |= Q -> forallM P |= Q.
+Proof.
+  intros r b in_b. apply r. apply in_b.
+Qed.
