coq/handwritten/CryptolToCoq/CompMExtra.v
@@ -1,0 +1,16 @@
+(***
+ *** Extra Proofs for CompM that Rely on SAWCorePrelude
+ ***)
+
+From CryptolToCoq Require Import SAWCorePrelude.
+From CryptolToCoq Require Export CompM.
+
+Lemma refinesM_either {A B C} (f:A -> CompM C) (g:B -> CompM C) eith P :
+  (forall a, eith = SAWCorePrelude.Left _ _ a -> f a |= P) ->
+  (forall b, eith = SAWCorePrelude.Right _ _ b -> g b |= P) ->
+  SAWCorePrelude.either _ _ _ f g eith |= P.
+Proof.
+  destruct eith; intros; simpl.
+  - apply H; reflexivity.
+  - apply H0; reflexivity.
+Qed.
